\exo{\ttps{} Opérations de fractions}{
    Calcul le résultat sous forme de fractions simplifié.
    \begin{enumerate}
        \item $\dfrac{-9}{2} + \dfrac{7}{5}
        = \nswr[3]{\dfrac{-9 \times 5}{2 \times 5} + \dfrac{7 \times 2}{5 \times 2}
        = \dfrac{-45}{10} + \dfrac{14}{10}
        = \dfrac{-31}{10}}$
        % \item $3 + \dfrac{5}{3}
        % = \nswr[3]{\dfrac{9}{3} + \dfrac{5}{3}
        % = \dfrac{14}{3}}$
        \item $\dfrac{1}{8} - \dfrac{5}{4} + \dfrac{-7}{6}
        = \nswr[5]{\dfrac{3}{24} - \dfrac{30}{24} + \dfrac{-28}{24}
        = \dfrac{3 - 30 - 28}{24}
        = \dfrac{-55}{24}}$
        \item $\dfrac{-8}{3} \times \dfrac{3}{4} \times \dfrac{5}{7}
        = \nswr[4]{\dfrac{-8 \times 3 \times 5}{3 \times 4 \times 7}
        = \dfrac{-120}{84}
        = \dfrac{-10}{7}}$
        \item $\dfrac{16}{21} \times \dfrac{35}{32}
        = \nswr[5]{\dfrac{16 \times 35}{21 \times 32}
        = \dfrac{\cancel{16} \times 5 \times \cancel{7}}{3 \times \cancel{7} \times \cancel{16} \times 2}
        = \dfrac{5}{6}}$
        \item $2 - \dfrac{3}{4} \times \dfrac{16}{9}
        = \nswr[6]{2 - \dfrac{48}{36}
        = 2 - \dfrac{48}{36}
        = \dfrac{72}{36} - \dfrac{48}{36}
        = \dfrac{24}{36}
        = \dfrac{24}{36}
        = \dfrac{2}{3}
        }$
        \item $\dfrac{5}{7} \div \dfrac{15}{2}
        = \nswr[4]{\dfrac{5}{7} \times \dfrac{2}{15}
        = \dfrac{\cancel{5} \times 2}{7 \times 3 \cancel{5}}
        = \dfrac{2}{21}}$
        % \item $\dfrac{2}{\dfrac{3}{5}}
        % = \nswr[3]{2 \times \dfrac{5}{3}
        % = \dfrac{10}{3}}$
    \end{enumerate}
}[\sesa{4}{2021}[][14]]