\expl{}{
    \multiColEnumerate{1}{
        \item $\frac{1}{2} - \frac{1}{4}
        = \nswr{\frac{2}{4} - \frac{1}{4}
        = \frac{2-1}{4} = \frac{1}{4}
        }$
        \item $\frac{2}{12} + \frac{2}{3}
        = \nswr{\frac{2}{12} + \frac{2\times4}{3\times4}
        = \frac{2}{12} + \frac{8}{12}
        = \frac{2+8}{12}
        = \frac{10}{12}
        }$
        \item $\frac{3}{5} + \frac{6}{7}
        = \nswr{\frac{3\times7}{5\times7} + \frac{6\times5}{7\times5}
        = \frac{21}{35} + \frac{30}{35}
        = \frac{21+30}{35} = \frac{51}{35}
        }$
        \item $\frac{12}{3} - \frac{6}{2}
        = \nswr{\frac{12\times2}{3\times2} - \frac{6\times3}{2\times3}
        = \frac{24}{6} - \frac{18}{6}
        = \frac{24-18}{6} = \frac{6}{6}
        }$
        \item $\frac{a}{b} + \frac{c}{d}
        = \nswr{\frac{a\times d}{b\times d} + \frac{c \times b}{d\times b}
        = \frac{ad}{bd} + \frac{cb}{bd}
        = \frac{ad+cb}{bd}
        }$
    }
}