\exo{15p167}{
    \multiColItemize{1}{
        \item $A = -5(x+2) = \nswr{-5 \times x + (- 5) \times 2 = -5x-10}$
        \item $B = -3(x-2) = \nswr{-3 \times x + (-3) \times (-2) = -3x + 6}$
        \item $C = x (x+3) = \nswr{x \times x + x \times 3 = x^2 + 3x}$
        \item $D = x (4-x) = \nswr{x \times 4 + x \times (-x) = 4x - x^2}$
        \item $E = -3x(x+4) = \nswr{-3x \times x + (-3x) \times 4 = -3x^2 - 12x}$
        \item $F = 2x (x - 7) = \nswr{2x \times x + 2x \times (-7) = 2x^2 - 14x}$
        \item $G = 6x (2x+1) = \nswr{6x \times 2x + 6x \times 1 = 12x^2 + 6x}$
        \item $H = -4x(5x-10) = \nswr{-4x \times 5x + (-4x) \times (-10) = -20x^2 + 40x}$
    }
}[\mi]