\exo{5p132}{
    \multiColItemize{1}{
        \item $A = \dfrac{-7}{3} \times \dfrac{5}{4} \times \dfrac{-1}{3}
        = \nswr{\dfrac{-7 \times 5 \times -1}{3 \times 4 \times 3}
        \dfrac{7 \times 5 \times 1}{3 \times 4 \times 3}
        = \dfrac{35}{36}}$
        \item $B = \dfrac{4}{3} \times \dfrac{-5}{7} \times \dfrac{-1}{3} \times (-5)
        = \nswr{\dfrac{4 \times -5 \times -1 \times -5}{3 \times 7 \times 3}
        = -\dfrac{4 \times 5 \times 1 \times 5}{3 \times 7 \times 3}
        = -\dfrac{100}{63}}$
    }
}[\mi]